Stack/StackLanguage.thy
@@ -2,8 +2,14 @@ theory StackLanguage
 imports "../Utilities/BasicComputation"
 begin
 
+datatype address = 
+  Constant int
+| Local nat
+| Argument nat
+
 datatype stack_instruction = 
   Add | Sub | Neg | Eq | Gt | Lt | And | Or | Not
+| Push address | Pop address
 | Print
 
 type_synonym stack_program = "code_label \<rightharpoonup> stack_instruction list \<times> code_label"
@@ -12,23 +18,42 @@ datatype stack_value =
   IntV int
 | Bool bool
 
-type_synonym stack_state = "stack_value list \<times> stack_instruction list \<times> code_label \<times> output" 
-  (* \<sigma>, \<pi>, s, \<omega> *)
+datatype frame = Frame "stack_value list" "stack_value list"
+
+type_synonym stack_state = 
+  "stack_value list \<times> frame list \<times> stack_instruction list \<times> code_label \<times> output" 
+  (* \<sigma>, \<phi>, \<pi>, s, \<omega> *)
 
 inductive eval_stack :: "stack_program \<Rightarrow> stack_state \<Rightarrow> stack_state \<Rightarrow> bool" where
-  evs_jump [simp]: "\<Pi> s = Some (\<pi>, s') \<Longrightarrow> eval_stack \<Pi> (\<sigma>, [], s, \<omega>) (\<sigma>, \<pi>, s', \<omega>)"
-| evs_add [simp]: "eval_stack \<Pi> (IntV i1 # IntV i2 # \<sigma>, Add # \<pi>, s, \<omega>) (IntV (i1 + i2) # \<sigma>, \<pi>, s, \<omega>)"
-| evs_sub [simp]: "eval_stack \<Pi> (IntV i1 # IntV i2 # \<sigma>, Sub # \<pi>, s, \<omega>) (IntV (i2 - i1) # \<sigma>, \<pi>, s, \<omega>)"
-| evs_neg [simp]: "eval_stack \<Pi> (IntV i1 # \<sigma>, Neg # \<pi>, s, \<omega>) (IntV (-i1) # \<sigma>, \<pi>, s, \<omega>)"
-| evs_eq [simp]: "eval_stack \<Pi> (IntV i1 # IntV i2 # \<sigma>, Eq # \<pi>, s, \<omega>) (Bool (i2 = i1) # \<sigma>, \<pi>, s, \<omega>)"
-| evs_gt [simp]: "eval_stack \<Pi> (IntV i1 # IntV i2 # \<sigma>, Gt # \<pi>, s, \<omega>) (Bool (i2 > i1) # \<sigma>, \<pi>, s, \<omega>)"
-| evs_lt [simp]: "eval_stack \<Pi> (IntV i1 # IntV i2 # \<sigma>, Lt # \<pi>, s, \<omega>) (Bool (i2 < i1) # \<sigma>, \<pi>, s, \<omega>)"
-| evs_and [simp]: "eval_stack \<Pi> (Bool i1 # Bool i2 # \<sigma>, And # \<pi>, s, \<omega>) (Bool (i2 \<and> i1) # \<sigma>, \<pi>, s, \<omega>)"
-| evs_or [simp]: "eval_stack \<Pi> (Bool i1 # Bool i2 # \<sigma>, Or # \<pi>, s, \<omega>) (Bool (i2 \<or> i1) # \<sigma>, \<pi>, s, \<omega>)"
-| evs_not [simp]: "eval_stack \<Pi> (Bool i1 # \<sigma>, Not # \<pi>, s, \<omega>) (Bool (\<not> i1) # \<sigma>, \<pi>, s, \<omega>)"
-| evs_print [simp]: "eval_stack \<Pi> (IntV i1 # \<sigma>, Print # \<pi>, s, \<omega>) (\<sigma>, \<pi>, s, i1 # \<omega>)"
+  evs_jump [simp]: "\<Pi> s = Some (\<pi>, s') \<Longrightarrow> eval_stack \<Pi> (\<sigma>, \<phi>, [], s, \<omega>) (\<sigma>, \<phi>, \<pi>, s', \<omega>)"
+| evs_add [simp]: "eval_stack \<Pi> (IntV i1 # IntV i2 # \<sigma>, \<phi>, Add # \<pi>, s, \<omega>) 
+    (IntV (i1 + i2) # \<sigma>, \<phi>, \<pi>, s, \<omega>)"
+| evs_sub [simp]: "eval_stack \<Pi> (IntV i1 # IntV i2 # \<sigma>, \<phi>, Sub # \<pi>, s, \<omega>) 
+    (IntV (i2 - i1) # \<sigma>, \<phi>, \<pi>, s, \<omega>)"
+| evs_neg [simp]: "eval_stack \<Pi> (IntV i1 # \<sigma>, \<phi>, Neg # \<pi>, s, \<omega>) (IntV (-i1) # \<sigma>, \<phi>, \<pi>, s, \<omega>)"
+| evs_eq [simp]: "eval_stack \<Pi> (IntV i1 # IntV i2 # \<sigma>, \<phi>, Eq # \<pi>, s, \<omega>) 
+    (Bool (i2 = i1) # \<sigma>, \<phi>, \<pi>, s, \<omega>)"
+| evs_gt [simp]: "eval_stack \<Pi> (IntV i1 # IntV i2 # \<sigma>, \<phi>, Gt # \<pi>, s, \<omega>) 
+    (Bool (i2 > i1) # \<sigma>, \<phi>, \<pi>, s, \<omega>)"
+| evs_lt [simp]: "eval_stack \<Pi> (IntV i1 # IntV i2 # \<sigma>, \<phi>, Lt # \<pi>, s, \<omega>) 
+    (Bool (i2 < i1) # \<sigma>, \<phi>, \<pi>, s, \<omega>)"
+| evs_and [simp]: "eval_stack \<Pi> (Bool i1 # Bool i2 # \<sigma>, \<phi>, And # \<pi>, s, \<omega>) 
+    (Bool (i2 \<and> i1) # \<sigma>, \<phi>, \<pi>, s, \<omega>)"
+| evs_or [simp]: "eval_stack \<Pi> (Bool i1 # Bool i2 # \<sigma>, \<phi>, Or # \<pi>, s, \<omega>) 
+    (Bool (i2 \<or> i1) # \<sigma>, \<phi>, \<pi>, s, \<omega>)"
+| evs_not [simp]: "eval_stack \<Pi> (Bool i1 # \<sigma>, \<phi>, Not # \<pi>, s, \<omega>) (Bool (\<not> i1) # \<sigma>, \<phi>, \<pi>, s, \<omega>)"
+| evs_push_c [simp]: "eval_stack \<Pi> (\<sigma>, \<phi>, Push (Constant i) # \<pi>, s, \<omega>) (IntV i # \<sigma>, \<phi>, \<pi>, s, \<omega>)"
+| evs_push_l [simp]: "eval_stack \<Pi> (\<sigma>, Frame as ls # \<phi>, Push (Local n) # \<pi>, s, \<omega>) 
+    (ls ! n # \<sigma>, \<phi>, \<pi>, s, \<omega>)"
+| evs_push_a [simp]: "eval_stack \<Pi> (\<sigma>, Frame as ls # \<phi>, Push (Argument n) # \<pi>, s, \<omega>) 
+    (as ! n # \<sigma>, \<phi>, \<pi>, s, \<omega>)"
+| evs_pop_l [simp]: "eval_stack \<Pi> (v # \<sigma>, Frame as ls # \<phi>, Pop (Local n) # \<pi>, s, \<omega>) 
+    (\<sigma>, Frame as (update_list ls v n) # \<phi>, \<pi>, s, \<omega>)"
+| evs_pop_a [simp]: "eval_stack \<Pi> (v # \<sigma>, Frame as ls # \<phi>, Pop (Argument n) # \<pi>, s, \<omega>) 
+    (\<sigma>, Frame (update_list as v n) ls # \<phi>, \<pi>, s, \<omega>)"
+| evs_print [simp]: "eval_stack \<Pi> (IntV i1 # \<sigma>, \<phi>, Print # \<pi>, s, \<omega>) (\<sigma>, \<phi>, \<pi>, s, i1 # \<omega>)"
 
 fun stack_output :: "stack_state \<Rightarrow> output" where
-  "stack_output (\<sigma>, \<pi>, s, \<omega>) = \<omega>"
+  "stack_output (\<sigma>, \<phi>, \<pi>, s, \<omega>) = \<omega>"
 
 end
