FlatStack/StackFlattener.thy
@@ -1,0 +1,76 @@
+theory StackFlattener
+imports Main
+begin
+
+primrec stack_to_mem :: "int list \<Rightarrow> (nat \<Rightarrow> int) \<Rightarrow> nat \<Rightarrow> int" where
+  "stack_to_mem [] \<mu> k = (if k = 0 then 0 else \<mu> k)"
+| "stack_to_mem (i # is) \<mu> k = (
+    if k = 0 then 1 + int (length is)
+    else if k = Suc (length is) then i
+    else stack_to_mem is \<mu> k)"
+
+lemma [simp]: "stack_to_mem \<sigma> \<mu> 0 = int (length \<sigma>)"
+  by (induction \<sigma>) simp_all
+
+lemma stack_same: "k > 0 \<Longrightarrow> k \<le> length \<sigma> \<Longrightarrow> stack_to_mem \<sigma> \<mu> k = stack_to_mem \<sigma> \<mu>' k"
+  by (induction \<sigma>) simp_all
+
+lemma [simp]: "k > length \<sigma> \<Longrightarrow> stack_to_mem \<sigma> \<mu> k = \<mu> k"
+  by (induction \<sigma>) simp_all
+
+lemma [simp]: "(stack_to_mem (a # \<sigma>) \<mu>)(nat (1 + int (length \<sigma>)) := b) = stack_to_mem (b # \<sigma>) \<mu>"
+  proof
+    fix x
+    show "((stack_to_mem (a # \<sigma>) \<mu>)(nat (1 + int (length \<sigma>)) := b)) x = stack_to_mem (b # \<sigma>) \<mu> x" 
+      by auto
+  qed
+
+lemma [simp]: "(stack_to_mem (i1 # \<sigma>) \<mu>)(0 := int (length \<sigma>)) = 
+    stack_to_mem \<sigma> (stack_to_mem (i1 # \<sigma>) \<mu>)"
+  proof
+    fix x
+    show "((stack_to_mem (i1 # \<sigma>) \<mu>)(0 := int (length \<sigma>))) x = 
+        stack_to_mem \<sigma> (stack_to_mem (i1 # \<sigma>) \<mu>) x" 
+      by (cases "x > length \<sigma>") (simp_all add: stack_same)
+  qed
+
+lemma [simp]: "(stack_to_mem (i1 # i2 # \<sigma>) \<mu>)(0 := 1 + int (length \<sigma>)) = 
+    stack_to_mem (i2 # \<sigma>) (stack_to_mem (i1 # i2 # \<sigma>) \<mu>)"
+  proof
+    fix x
+    show "((stack_to_mem (i1 # i2 # \<sigma>) \<mu>)(0 := 1 + int (length \<sigma>))) x = 
+        stack_to_mem (i2 # \<sigma>) (stack_to_mem (i1 # i2 # \<sigma>) \<mu>) x"
+      by (cases "x > length \<sigma>") (simp_all add: stack_same)
+  qed
+
+lemma [simp]: "(stack_to_mem \<sigma> \<mu>)(0 := int (length \<sigma>) + 1, nat (int (length \<sigma>) + 1) := d) = 
+    stack_to_mem (d # \<sigma>) \<mu>"
+  proof
+    fix x
+    show "((stack_to_mem \<sigma> \<mu>)(0 := int (length \<sigma>) + 1, nat (int (length \<sigma>) + 1) := d)) x = 
+        stack_to_mem (d # \<sigma>) \<mu> x" by auto
+  qed
+
+lemma [simp]: "n < length \<sigma> \<Longrightarrow> stack_to_mem \<sigma> \<mu> (nat (int (length \<sigma>) - int n)) = \<sigma> ! n"
+  proof (induction \<sigma> arbitrary: n)
+  case Nil
+    thus ?case by simp
+  next case Cons
+    thus ?case by (induction n) fastforce+
+  qed
+
+lemma [simp]: "n < length \<sigma> \<Longrightarrow> (stack_to_mem \<sigma> \<mu>)(nat (int (length \<sigma>) - int n) := d) = 
+    stack_to_mem (\<sigma>[n := d]) \<mu>"
+  proof
+    fix x
+    assume "n < length \<sigma>"
+    thus "((stack_to_mem \<sigma> \<mu>)(nat (int (length \<sigma>) - int n) := d)) x = stack_to_mem (\<sigma>[n := d]) \<mu> x"
+      proof (induction \<sigma> arbitrary: n)
+      case Nil
+        thus ?case by simp
+      next case Cons
+        thus ?case by (induction n) fastforce+
+      qed
+  qed
+
+end
